hax-lib/proof-libs/lean/Hax/USize64.lean
@@ -1,27 +1,32 @@
 import Hax.MissingLean.Init.Data.UInt.Lemmas
+import Lean.Meta.Tactic.Simp.BuiltinSimprocs.UInt
 
 open Std
 open Nat
 
-def USize64 := UInt64
+structure USize64 where ofUInt64 :: toUInt64 : UInt64
 
-def USize64.size : Nat := UInt64.size
-def USize64.ofNat (n : Nat) : USize64 := UInt64.ofNat n
-def USize64.toNat (n : USize64) : Nat := UInt64.toNat n
-def USize64.ofBitVec (n : BitVec 64) : USize64 := UInt64.ofBitVec n
-def USize64.toBitVec (n : USize64) : BitVec 64 := UInt64.toBitVec n
-def USize64.toFin (n : USize64) : Fin USize64.size := UInt64.toFin n
+@[reducible] def USize64.size : Nat := UInt64.size
+def USize64.ofNat (n : Nat) : USize64 := ⟨UInt64.ofNat n⟩
+def USize64.toNat (n : USize64) : Nat := UInt64.toNat n.toUInt64
+def USize64.ofBitVec (n : BitVec 64) : USize64 := ⟨UInt64.ofBitVec n⟩
+def USize64.toBitVec (n : USize64) : BitVec 64 := UInt64.toBitVec n.toUInt64
+def USize64.toFin (n : USize64) : Fin USize64.size := UInt64.toFin n.toUInt64
 
-def USize64.ofNatLT (n : @& Nat) (h : LT.lt n USize64.size) : USize64 := UInt64.ofNatLT n h
+def USize64.ofNatLT (n : @& Nat) (h : LT.lt n USize64.size) : USize64 := ⟨UInt64.ofNatLT n h⟩
 
-def USize64.decEq (a b : USize64) : Decidable (Eq a b) := UInt64.decEq a b
+def USize64.decEq (a b : USize64) : Decidable (Eq a b) := by cases a; cases b; simp; infer_instance
+
+namespace USize64
 
 instance : DecidableEq USize64 := USize64.decEq
 
 instance : Inhabited USize64 where
   default := USize64.ofNatLT 0 (of_decide_eq_true rfl)
 
-instance {n} : OfNat USize64 n := by unfold USize64; infer_instance
+instance {n} : OfNat USize64 n := ⟨⟨OfNat.ofNat n⟩⟩
+
+end USize64
 
 @[inline] def USize64.ofFin (a : Fin USize64.size) : USize64 := ⟨⟨a⟩⟩
 
@@ -30,23 +35,20 @@ def USize64.ofInt (x : Int) : USize64 := ofNat (x % 2 ^ 64).toNat
 @[simp] theorem USize64.le_size : 2 ^ 32 ≤ USize64.size := by simp [USize64.size, UInt64.size]
 @[simp] theorem USize64.size_le : USize64.size ≤ 2 ^ 64 := by simp [USize64.size, UInt64.size]
 
-protected def USize64.add (a b : USize64) : USize64 := ⟨a.toBitVec + b.toBitVec⟩
-protected def USize64.sub (a b : USize64) : USize64 := ⟨a.toBitVec - b.toBitVec⟩
-protected def USize64.mul (a b : USize64) : USize64 := ⟨a.toBitVec * b.toBitVec⟩
-protected def USize64.div (a b : USize64) : USize64 := ⟨BitVec.udiv a.toBitVec b.toBitVec⟩
-protected def USize64.pow (x : USize64) (n : Nat) : USize64 :=
-  match n with
-  | 0 => 1
-  | n + 1 => USize64.mul (USize64.pow x n) x
-protected def USize64.mod (a b : USize64) : USize64 := ⟨BitVec.umod a.toBitVec b.toBitVec⟩
+protected def USize64.add (a b : USize64) : USize64 := ⟨a.toUInt64 + b.toUInt64⟩
+protected def USize64.sub (a b : USize64) : USize64 := ⟨a.toUInt64 - b.toUInt64⟩
+protected def USize64.mul (a b : USize64) : USize64 := ⟨a.toUInt64 * b.toUInt64⟩
+protected def USize64.div (a b : USize64) : USize64 := ⟨a.toUInt64 / b.toUInt64⟩
+protected def USize64.pow (x : USize64) (n : Nat) : USize64 := ⟨x.toUInt64 ^ n⟩
+protected def USize64.mod (a b : USize64) : USize64 := ⟨a.toUInt64 % b.toUInt64⟩
 
-protected def USize64.land (a b : USize64) : USize64 := ⟨a.toBitVec &&& b.toBitVec⟩
-protected def USize64.lor (a b : USize64) : USize64 := ⟨a.toBitVec ||| b.toBitVec⟩
-protected def USize64.xor (a b : USize64) : USize64 := ⟨a.toBitVec ^^^ b.toBitVec⟩
-protected def USize64.shiftLeft (a b : USize64) : USize64 := ⟨a.toBitVec <<< (USize64.mod b 64).toBitVec⟩
-protected def USize64.shiftRight (a b : USize64) : USize64 := ⟨a.toBitVec >>> (USize64.mod b 64).toBitVec⟩
-protected def USize64.lt (a b : USize64) : Prop := a.toBitVec < b.toBitVec
-protected def USize64.le (a b : USize64) : Prop := a.toBitVec ≤ b.toBitVec
+protected def USize64.land (a b : USize64) : USize64 := ⟨a.toUInt64 &&& b.toUInt64⟩
+protected def USize64.lor (a b : USize64) : USize64 := ⟨a.toUInt64 ||| b.toUInt64⟩
+protected def USize64.xor (a b : USize64) : USize64 := ⟨a.toUInt64 ^^^ b.toUInt64⟩
+protected def USize64.shiftLeft (a b : USize64) : USize64 := ⟨a.toUInt64 <<< (USize64.mod b 64).toUInt64⟩
+protected def USize64.shiftRight (a b : USize64) : USize64 := ⟨a.toUInt64 >>> (USize64.mod b 64).toUInt64⟩
+protected def USize64.lt (a b : USize64) : Prop := a.toUInt64 < b.toUInt64
+protected def USize64.le (a b : USize64) : Prop := a.toUInt64 ≤ b.toUInt64
 
 instance : Add USize64       := ⟨USize64.add⟩
 instance : Sub USize64       := ⟨USize64.sub⟩
@@ -54,14 +56,14 @@ instance : Mul USize64       := ⟨USize64.mul⟩
 instance : Pow USize64 Nat   := ⟨USize64.pow⟩
 instance : Mod USize64       := ⟨USize64.mod⟩
 
-instance : HMod USize64 Nat USize64 := by unfold USize64; infer_instance
+instance : HMod USize64 Nat USize64 := ⟨fun x n => ⟨x.toUInt64 % n⟩⟩
 
 instance : Div USize64       := ⟨USize64.div⟩
 instance : LT USize64        := ⟨USize64.lt⟩
 instance : LE USize64        := ⟨USize64.le⟩
 
-protected def USize64.complement (a : USize64) : USize64 := ⟨~~~a.toBitVec⟩
-protected def USize64.neg (a : USize64) : USize64 := ⟨-a.toBitVec⟩
+protected def USize64.complement (a : USize64) : USize64 := ⟨~~~a.toUInt64⟩
+protected def USize64.neg (a : USize64) : USize64 := ⟨-a.toUInt64⟩
 
 instance : Complement USize64 := ⟨USize64.complement⟩
 instance : Neg USize64 := ⟨USize64.neg⟩
@@ -81,8 +83,7 @@ def UInt16.toUSize64 (a : UInt16) : USize64 :=
 def USize64.toUInt16 (a : USize64) : UInt16 := a.toNat.toUInt16
 def UInt32.toUSize64 (a : UInt32) : USize64 := USize64.ofNat32 a.toBitVec.toNat a.toBitVec.isLt
 def USize64.toUInt32 (a : USize64) : UInt32 := a.toNat.toUInt32
-def UInt64.toUSize64 (a : UInt64) : USize64 := a.toNat.toUInt64
-def USize64.toUInt64 (a : USize64) : UInt64 := a
+def UInt64.toUSize64 (a : UInt64) : USize64 := ⟨a⟩
 def Bool.toUSize64 (b : Bool) : USize64 := if b then 1 else 0
 def USize64.decLt (a b : USize64) : Decidable (a < b) :=
   inferInstanceAs (Decidable (a.toBitVec < b.toBitVec))
@@ -182,7 +183,6 @@ theorem USize64.toNat_ofNat_of_lt {n : Nat} (h : n < size) : toNat (OfNat.ofNat 
 
 namespace Lean.Grind
 
-
 instance : ToInt USize64 (.uint 64) where
   toInt x := (x.toNat : Int)
   toInt_inj x y w := sorry -- USize64.toNat_inj.mp (Int.ofNat_inj.mp w)
@@ -202,8 +202,7 @@ instance : ToInt.Add USize64 (.uint 64) where
 instance : ToInt.Mul USize64 (.uint 64) where
   toInt_mul x y := sorry -- by simp
 
--- The `ToInt.Pow` instance is defined in `Init.GrindInstances.Ring.UInt`,
--- as it is convenient to use the ring structure.
+instance : ToInt.Pow USize64 (.uint 64) := by sorry
 
 instance : ToInt.Mod USize64 (.uint 64) where
   toInt_mod x y := sorry -- by simp
@@ -217,4 +216,129 @@ instance : ToInt.LE USize64 (.uint 64) where
 instance : ToInt.LT USize64 (.uint 64) where
   lt_iff x y := sorry -- by simpa using USize64.lt_iff_toBitVec_lt
 
+
+@[expose]
+def USize64.natCast : NatCast USize64 where
+  natCast x := USize64.ofNat x
+
+@[expose]
+def USize64.intCast : IntCast USize64 where
+  intCast x := USize64.ofInt x
+
+attribute [local instance] USize64.natCast USize64.intCast in
+instance : CommRing USize64 where
+  nsmul := ⟨(· * ·)⟩
+  zsmul := ⟨(· * ·)⟩
+  add_assoc := sorry -- UInt64.add_assoc
+  add_comm := sorry -- UInt64.add_comm
+  add_zero := sorry -- UInt64.add_zero
+  neg_add_cancel := sorry -- UInt64.add_left_neg
+  mul_assoc := sorry -- UInt64.mul_assoc
+  mul_comm := sorry -- UInt64.mul_comm
+  mul_one := sorry -- UInt64.mul_one
+  one_mul := sorry -- UInt64.one_mul
+  left_distrib _ _ _ := sorry -- UInt64.mul_add
+  right_distrib _ _ _ := sorry -- UInt64.add_mul
+  zero_mul _ := sorry -- UInt64.zero_mul
+  mul_zero _ := sorry -- UInt64.mul_zero
+  sub_eq_add_neg := sorry -- UInt64.sub_eq_add_neg
+  pow_zero := sorry -- UInt64.pow_zero
+  pow_succ := sorry -- UInt64.pow_succ
+  ofNat_succ x := sorry -- UInt64.ofNat_add x 1
+  intCast_neg := sorry -- UInt64.ofInt_neg
+  intCast_ofNat := sorry -- UInt64.intCast_ofNat
+  neg_zsmul i a := by
+    -- change (-i : Int) * a = - (i * a)
+    sorry -- simp [UInt64.intCast_neg, UInt64.neg_mul]
+  zsmul_natCast_eq_nsmul n a := sorry -- congrArg (· * a) (USize64.intCast_ofNat _)
+
+instance : IsCharP USize64 18446744073709551616 := IsCharP.mk' _ _
+  (ofNat_eq_zero_iff := fun x => by
+    have : OfNat.ofNat x = USize64.ofNat x := rfl
+    sorry -- simp [this, USize64.ofNat_eq_iff_mod_eq_toNat]
+    )
+
+-- Verify we can derive the instances showing how `toInt` interacts with operations:
+example : ToInt.Add USize64 (.uint 64) := inferInstance
+example : ToInt.Neg USize64 (.uint 64) := {
+  toInt_neg := sorry
+}
+example : ToInt.Sub USize64 (.uint 64) := {
+  toInt_sub := sorry
+}
+
+
 end Lean.Grind
+
+
+namespace USize64
+open Lean Meta Simp
+
+instance : ToExpr USize64 where
+  toTypeExpr := mkConst ``USize64
+  toExpr a :=
+    let r := mkRawNatLit a.toNat
+    mkApp3 (.const ``OfNat.ofNat [0]) (mkConst ``USize64) r
+      (.app (.const ``USize64.instOfNat []) r)
+
+def fromExpr (e : Expr) : SimpM (Option USize64) := do
+  let some (n, _) ← getOfNatValue? e `USize64 | return none
+  return USize64.ofNat n
+
+@[inline] def reduceBin (declName : Name) (arity : Nat) (op : USize64 → USize64 → USize64) (e : Expr) : SimpM DStep := do
+  unless e.isAppOfArity declName arity do return .continue
+  let some n ← (fromExpr e.appFn!.appArg!) | return .continue
+  let some m ← (fromExpr e.appArg!) | return .continue
+  return .done <| toExpr (op n m)
+
+@[inline] def reduceBinPred (declName : Name) (arity : Nat) (op : USize64 → USize64 → Bool) (e : Expr) : SimpM Step := do
+  unless e.isAppOfArity declName arity do return .continue
+  let some n ← (fromExpr e.appFn!.appArg!) | return .continue
+  let some m ← (fromExpr e.appArg!) | return .continue
+  evalPropStep e (op n m)
+
+@[inline] def reduceBoolPred (declName : Name) (arity : Nat) (op : USize64 → USize64 → Bool) (e : Expr) : SimpM DStep := do
+  unless e.isAppOfArity declName arity do return .continue
+  let some n ← (fromExpr e.appFn!.appArg!) | return .continue
+  let some m ← (fromExpr e.appArg!) | return .continue
+  return .done <| toExpr (op n m)
+
+dsimproc [simp, seval] reduceAdd ((_ + _ : USize64)) := reduceBin ``HAdd.hAdd 6 (· + ·)
+dsimproc [simp, seval] reduceMul ((_ * _ : USize64)) := reduceBin ``HMul.hMul 6 (· * ·)
+dsimproc [simp, seval] reduceSub ((_ - _ : USize64)) := reduceBin ``HSub.hSub 6 (· - ·)
+dsimproc [simp, seval] reduceDiv ((_ / _ : USize64)) := reduceBin ``HDiv.hDiv 6 (· / ·)
+dsimproc [simp, seval] reduceMod ((_ % _ : USize64)) := reduceBin ``HMod.hMod 6 (· % ·)
+
+simproc [simp, seval] reduceLT  (( _ : USize64) < _)  := reduceBinPred ``LT.lt 4 (. < .)
+simproc [simp, seval] reduceLE  (( _ : USize64) ≤ _)  := reduceBinPred ``LE.le 4 (. ≤ .)
+simproc [simp, seval] reduceGT  (( _ : USize64) > _)  := reduceBinPred ``GT.gt 4 (. > .)
+simproc [simp, seval] reduceGE  (( _ : USize64) ≥ _)  := reduceBinPred ``GE.ge 4 (. ≥ .)
+simproc [simp, seval] reduceEq  (( _ : USize64) = _)  := reduceBinPred ``Eq 3 (. = .)
+simproc [simp, seval] reduceNe  (( _ : USize64) ≠ _)  := reduceBinPred ``Ne 3 (. ≠ .)
+dsimproc [simp, seval] reduceBEq  (( _ : USize64) == _)  := reduceBoolPred ``BEq.beq 4 (. == .)
+dsimproc [simp, seval] reduceBNe  (( _ : USize64) != _)  := reduceBoolPred ``bne 4 (. != .)
+
+dsimproc [simp, seval] reduceOfNatLT (USize64.ofNatLT _ _) := fun e => do
+  unless e.isAppOfArity `USize64.ofNatLT 2 do return .continue
+  let some value ← Nat.fromExpr? e.appFn!.appArg! | return .continue
+  let value := USize64.ofNat value
+  return .done <| toExpr value
+
+dsimproc [simp, seval] reduceOfNat (USize64.ofNat _) := fun e => do
+  unless e.isAppOfArity `USize64.ofNat 1 do return .continue
+  let some value ← Nat.fromExpr? e.appArg! | return .continue
+  let value := USize64.ofNat value
+  return .done <| toExpr value
+
+dsimproc [simp, seval] reduceToNat (USize64.toNat _) := fun e => do
+  unless e.isAppOfArity `USize64.toNat 1 do return .continue
+  let some v ← (fromExpr e.appArg!) | return .continue
+  let n := USize64.toNat v
+  return .done <| toExpr n
+
+/-- Return `.done` for UInt values. We don't want to unfold in the symbolic evaluator. -/
+dsimproc [seval] isValue ((OfNat.ofNat _ : USize64)) := fun e => do
+  unless (e.isAppOfArity ``OfNat.ofNat 3) do return .continue
+  return .done e
+
+end USize64
